Checkpoint (machinery for reasoning about StateT and Except T)
Originally https://github.com/dfinity-lab/ic-ref/commit/9f27ff59a40949d3c3db0133a1b9bfa2962e0d93

proofs/theories/IC/Ref.v
@@ -7,6 +7,7 @@ Require Import IC.Types.
 Require Import Data.Map.Internal.
 
 Import GHC.Base.
+Import Data.Either.
 Import GHC.Base.Notations.
 Import List.Notations.
 
@@ -27,6 +28,41 @@ Ltac destruct_match :=
     let Heq := fresh "Heq" in
     destruct a eqn:Heq
   end.
+
+(** This tactic finds a [let x := rhs in body] anywhere in the goal,
+    and moves it into the context, without zeta-reducing it. *)
+Ltac find_let e k :=
+  lazymatch e with 
+  (** LY: It seems that there is a bug in Coq about variable binding.
+      This is a temporary fix. *)
+  | let _go := ?rhs in ?body => k _go rhs body
+  | ?e1 ?e2 =>
+    find_let e1 ltac:(fun x rhs body => k x rhs uconstr:(body e2)) ||
+    find_let e2 ltac:(fun x rhs body => k x rhs uconstr:(e1 body))
+  | _ => fail
+  end.
+Ltac float_let :=
+  lazymatch goal with |- ?goal =>
+    find_let goal ltac:(fun x rhs body =>
+      let goal' := uconstr:(let x := rhs in let _go := x in body) in
+      (change goal'; do 2 intro; subst) || fail 1000 "Failed to change to" goal'
+    )
+  end.
+
+(* NB, this does not work:
+Ltac float_let :=
+  lazymatch goal with |-  context C [let x := ?rhs in ?body] =>
+    let goal' := context C[body] in
+    change (let x := rhs in goal'); intro
+  end.
+*)
+
+(** Common subexpression elimination *)
+Ltac cse_let :=
+      repeat lazymatch goal with
+        [ x := ?rhs, x0 := ?rhs |- _ ] =>
+          change x0 with x in *;clear x0
+        end.
 
 
 (* Lemmas about State *)
@@ -105,6 +141,22 @@ Lemma runState_return:
   forall S A (x : A) (s : S), runState (return_ x) s = (x,s).
 Proof. intros. reflexivity. Qed.
 
+
+Lemma runState_fmap:
+  forall S A B(f : A -> B) (m : State S A) (s : S),
+  runState (fmap f m) s = 
+    let (x, s') := runState m s in
+    (f x, s').
+Proof. intros.
+  destruct m as [m].
+  unfold runState, Base.op_z2218U__, runIdentity, runStateT.
+  unfold fmap, Functor__StateT, fmap__, Lazy.Functor__StateT_fmap.
+  unfold fmap, Functor__Identity, fmap__, Identity.Functor__Identity_fmap.
+  unfold runStateT.
+  destruct (m s) as [ms].
+  reflexivity.
+Qed.
+
 Lemma runState_bind:
   forall S A B (m1 : State S A) (m2 : A -> State S B) (s : S),
   runState (m1 >>= m2) s = 
@@ -154,6 +206,175 @@ Proof.
   unfold runState, Base.op_z2218U__, runIdentity, runStateT in H. 
   destruct (m1 s), (m2 s).
   congruence.
+Qed.
+
+
+Definition SP {a} {s} (P Q : s -> Prop) (R : a -> Prop) (act : State s a) :=
+  forall s, P s -> Q (snd (runState act s)) /\ R (fst (runState act s)).
+
+Definition StateInvariant {a} {s} (P : s -> Prop) (act : State s a) :=
+  SP P P (fun _ => True) act.
+
+
+Lemma SP_snd_runState:
+  forall {a s} (P P' : s -> Prop) (R : a -> Prop) (act : State s a) (x : s),
+  SP P P' R act ->
+  P x ->
+  P' (snd (runState act x)).
+Proof.
+  intros.
+  unfold SP in H.
+  apply H. assumption.
+Qed.
+
+Lemma SP_return:
+  forall {a s} (P : s -> Prop) (Q : a -> Prop) (x : a),
+  Q x -> SP P P Q (return_ x).
+Proof. intros. intros s0 HP. split; assumption. Qed.
+
+
+Lemma SP_put:
+  forall {s} (P P' : s -> Prop) x,
+  P' x ->
+  SP P P' (fun _ => True) (put x).
+Proof. intros. intros s0 _. split; [ apply H | trivial ]. Qed.
+
+Lemma SP_get:
+  forall {s} (P : s -> Prop) (R : s -> Prop),
+  (forall s, P s -> R s) ->
+  SP P P R get.
+Proof. intros. intros s0 H2. split; auto. Qed.
+
+Lemma SP_gets:
+  forall {s a} (P : s -> Prop) P' (f : s -> a),
+  SP P P (fun x => P' (f x)) get ->
+  SP P P P' (gets f).
+Proof. intros. intros s0 H1. apply H. assumption. Qed.
+
+Lemma SP_modify:
+  forall {S} (P : S -> Prop) (P' : S -> Prop) (f : S -> S),
+  (forall s, P s -> P' (f s)) ->
+  SP P P' (fun _ => True) (modify f).
+Proof. intros. intros s0 H1. split; auto.
+ unfold modify. rewrite runState_state. simpl. auto. Qed.
+
+Lemma SP_bind:
+  forall {a b s} P P' P'' R R' (act1 : State s a) (act2 : a -> State s b),
+  SP P P' R act1 ->
+  (forall x, R x -> SP P' P'' R' (act2 x)) ->
+  SP P P'' R' (act1 >>= act2).
+Proof.
+  intros ?????????? H1 H2.
+  intros s0 H.
+  simpl.
+  rewrite runState_bind.
+  expand_pairs.
+  eapply H2; apply H1; assumption.
+Qed.
+
+Lemma SP_fmap:
+  forall {a b s} P P' R (f : a -> b) (act : State s a),
+  SP P P' (fun x => R (f x)) act ->
+  SP P P' R (fmap f act).
+Proof.
+  intros.
+  intros s0 H1.
+  rewrite runState_fmap.
+  expand_pairs. simpl.
+  apply H. assumption.
+Qed.
+
+Lemma StateInvariant_return:
+  forall {a s} (P : s -> Prop) (x : a),
+  StateInvariant P (return_ x).
+Proof. intros. apply SP_return. trivial. Qed.
+
+Lemma StateInvariant_get:
+  forall {s} (P : s -> Prop),
+  StateInvariant P get.
+Proof. intros. eapply SP_get. split. Qed.
+
+
+Lemma StateInvariant_gets:
+  forall {b s} (P : s -> Prop) (f : s -> b),
+  StateInvariant P (gets f).
+Proof. intros. apply SP_gets. apply StateInvariant_get. Qed.
+
+
+Lemma StateInvariant_bind:
+  forall {a b s} P (act1 : State s a) (act2 : a -> State s b),
+  StateInvariant P act1 ->
+  (forall x, StateInvariant P (act2 x)) ->
+  StateInvariant P (act1 >>= act2).
+Proof.
+  intros. eapply SP_bind.
+  * apply H.
+  * intros ? _.  apply H0.
+Qed.
+
+Lemma StateInvariant_bind_return: (*  acommon pattern *)
+  forall {a b s} P (act1 : State s a) (f : a -> b),
+  StateInvariant P act1 ->
+  StateInvariant P (act1 >>= (fun x => return_ (f x))).
+Proof.
+  intros.
+  apply StateInvariant_bind.
+  * apply H.
+  * intro. apply StateInvariant_return.
+Qed.
+
+Lemma StateInvarinat_fmap:
+  forall {a b s} P (f : a -> b) (act : State s a),
+  StateInvariant P act ->
+  StateInvariant P (fmap f act).
+Proof.
+  intros.
+  apply SP_fmap.
+  apply H.
+Qed.
+
+
+Lemma StateInvariant_liftA2:
+  forall {a b c s} P (f : a -> b -> c) (act1 : State s a) (act2 : State s b),
+  StateInvariant P act1 ->
+  StateInvariant P act2 ->
+  StateInvariant P (liftA2 f act1 act2).
+Proof.
+  intros.
+  rewrite applicative_liftA2.
+  rewrite monad_applicative_ap.
+  unfold ap.
+  apply StateInvariant_bind; [|intros; apply StateInvariant_bind; intros].
+  apply StateInvarinat_fmap; assumption.
+  assumption.
+  apply StateInvariant_return.
+Qed.
+
+Lemma StateInvariant_mapM:
+  forall {a b s} P (act : a -> State s b) (xs : list a),
+  (forall x, In x xs -> StateInvariant P (act x)) ->
+  StateInvariant P (Traversable.mapM act xs).
+Proof.
+  intros ?????? Hact.
+  unfold Traversable.mapM, Traversable.Traversable__list, Traversable.mapM__,
+         Traversable.Traversable__list_mapM, Traversable.Traversable__list_traverse.
+  induction xs.
+  * apply StateInvariant_return.
+  * simpl.
+    apply StateInvariant_liftA2.
+    - apply Hact. left. reflexivity.
+    - apply IHxs. intros x Hin. apply Hact. right. assumption.
+Qed.
+
+Lemma StateInvariant_forM:
+  forall {a b s} P (act : a -> State s b) (xs : list a),
+  (forall x, In x xs -> StateInvariant P (act x)) ->
+  StateInvariant P (Traversable.forM xs act).
+Proof.
+  intros.
+  unfold Traversable.forM, flip.
+  apply StateInvariant_mapM.
+  assumption.
 Qed.
 
 
@@ -213,6 +434,28 @@ Lemma onReject_return:
 Proof. intros. apply state_extensionality. intro. reflexivity. Qed. 
 
 
+Lemma throwE_bind:
+  forall M E A B (e : E) (act : A -> ExceptT E M B) `{MLM : MonadLaws M},
+  (throwE e >>= act) = throwE e.
+Proof.
+  intros.
+  unfold throwE, Base.op_z2218U__.
+  unfold op_zgzgze__, Monad__ExceptT, op_zgzgze____, Monad__ExceptT_op_zgzgze__.
+  simpl.
+  rewrite monad_left_id.
+  reflexivity.
+Qed.
+
+Lemma throwE_bind':
+  forall A B e (act : A -> RM B),
+  (throwE e >>= act) = throwE e.
+Proof.
+  intros.
+  (* Why doesn't type class resolution work here without help.? *)
+  apply throwE_bind with (ApplicativeLaws0 := instance_ApplicativeLaws_StateT).
+  typeclasses eauto.
+Qed.
+
 Lemma onReject_throwE:
   forall A B f x (h : RM A),
   (onReject f ((throwE x : RM B) >> h)) = f x.
@@ -224,6 +467,94 @@ Lemma pure_then_RM:
 (* This should follow from the MonadLaws *)
 Proof. intros. reflexivity. Qed.
 
+Definition PRight {A B} P (x : Either A B) := match x with
+  | Left e => True
+  | Right y => P y
+  end.
+
+Definition ESP {S A E} (P : S -> Prop) (R : A -> Prop) (act : ExceptT E (State S) A) :=
+  SP P P (PRight R) (runExceptT act).
+
+Lemma ESP_return:
+  forall {s e a} (P : s -> Prop) (R : a -> Prop) (x : a),
+  R x -> (ESP (E := e)) P R (return_ x).
+Proof. intros. apply SP_return. trivial. Qed.
+
+Lemma ESP_bind:
+  forall {s e a b} (P : s -> Prop) R (R' : b -> Prop)
+  (act1 : ExceptT e (State s) a) act2,
+  ESP P R act1 ->
+  (forall (x : a), R x -> ESP P R' (act2 x)) ->
+  ESP P R' (act1 >>= act2).
+Proof.
+  intros.
+  unfold ESP in *.
+  destruct act1 as [act1].
+  unfold runExceptT in *.
+  simpl in *.
+  eapply SP_bind.
+  * apply H.
+  * intros. unfold PRight in H1.
+    destruct x.
+    - apply SP_return. trivial.
+    - apply H0. assumption.
+Qed.
+
+Lemma ESP_then:
+  forall {s e a b} (P : s -> Prop) (R : b -> Prop)
+  (act1 : ExceptT e (State s) a) act2,
+  ESP P (fun _ => True) act1 ->
+  ESP P R act2 ->
+  ESP P R (act1 >> act2).
+Proof.
+  intros.
+  rewrite monad_then.
+  eapply ESP_bind.
+  apply H.
+  intros.
+  apply H0.
+Qed.
+
+
+Lemma ESP_throwE:
+  forall {s e a} (P : s -> Prop) (R : a -> Prop) (x : e),
+  ESP P R (throwE x).
+Proof. intros. apply SP_return. constructor. Qed.
+
+
+Lemma ESP_liftRM:
+  forall {A P R} (act : M A),
+  SP P P R act ->
+  ESP P R (liftRM act).
+Proof.
+  intros.
+  unfold ESP.
+  unfold liftRM, Class.lift, MonadTrans__ExceptT, Class.lift__, liftM,
+    Except.MonadTrans__ExceptT_lift, liftM.
+  simpl.
+  eapply SP_bind.
+  * apply H.
+  * intros. apply SP_return. apply H0.
+Qed.
+
+Lemma SP_onReject:
+  forall {A} P R
+  (act : RM A) f,
+  (forall e, SP P P R (f e)) ->
+  ESP P R act ->
+  SP P P R (onReject f act).
+Proof.
+  intros.
+  unfold onReject.
+  eapply SP_bind.
+  * apply H0.
+  * intros.
+    unfold PRight in H1.
+    destruct x.
+    - apply H.
+    - apply SP_return. assumption.
+Qed.
+
 
 Definition ICInvariant Q P :=
   P initialIC /\
@@ -232,9 +563,7 @@ Definition ICInvariant Q P :=
     Q pk r ->
     evalState (authAsyncRequest pk r) s0 = true ->
     P (execState (submitRequest rid r) s0)) /\
-  (forall s0,
-    P s0 ->
-    P (execState runStep s0)).
+  StateInvariant P runStep.
 
 
 Definition any_request (pk : Blob) (r : AsyncRequest) := True.
@@ -243,6 +572,7 @@ Theorem no_empty_canister_id :
   ICInvariant any_request (fun s =>
     member (Mk_EntityId nil) (canisters s) = false).
 Proof.
+  set (P := fun s : IC => member (Mk_EntityId nil) (canisters s) = false).
   split; [|split].
   * reflexivity.
   * intros.
@@ -256,74 +586,63 @@ Proof.
     + destruct s0. assumption.
   * intros.
     unfold runStep.
-    unfold nextReceived.
-    unfold execState.
-    rewrite runState_gets.
-    destruct_match.
-    + destruct p as [rid ar].
-      rewrite runState_then.
-      rewrite runState_return.
-      simpl.
+    repeat (apply StateInvariant_bind; [|intros; destruct x as [[rid ar]|]]).
+    + unfold nextReceived.
+      apply StateInvariant_gets.
+      (* Somehow pass information about ar down? *)
+    + apply StateInvariant_bind; [|intros; apply StateInvariant_return].
       unfold processRequest.
+      unfold op_zezlzl__.
+      apply StateInvariant_bind; [|intros; apply SP_modify; destruct s; simpl; auto].
       destruct_match.
-      - unfold op_zezlzl__.
-        (* TODO: This duplicates the continuation. How to common up? *)
-        destruct_match.
-        ** rewrite runState_bind.
-           rewrite onReject_liftRM_bind.
-           rewrite runState_gets.
-           rewrite onReject_liftRM_bind.
-           rewrite runState_gets.
-           match goal with | [ |- context[when ?P] ] => destruct P eqn:Hwhen end.
-           ++ unfold when.
-              unfold reject.
-              rewrite onReject_throwE.
-              simpl.
-              destruct s0. simpl. assumption.
-           ++ unfold when. rewrite pure_then_RM.
-              rewrite onReject_liftRM_then.
-              unfold createEmptyCanister.
-              rewrite runState_then.
-              unfold modify. rewrite runState_state.
-              unfold snd.
-              rewrite onReject_return, runState_return.
-              unfold setReqStatus.
-              unfold modify. rewrite runState_state.
-              unfold Base.op_z2218U__ in *.
-              destruct s0.
-              simpl.
-              (* now need theory about member and insert *)
-              (* and that freshid is not nil *)
+      - (* Create request *)
+        apply SP_onReject.
+        intro; apply SP_return; trivial.
+        set (R' := fun new_id => not (new_id = Mk_EntityId nil)).
+        apply ESP_bind with (R := R').
+        ** destruct_match.
+           -- (* System picks *)
+              apply ESP_liftRM.
+              apply SP_gets.
+              apply SP_get.
+              intros.
+              subst R'; unfold op_z2218U__; simpl.
+              admit. (* fresh id is not nil *)
+           -- (* Forced choice *)
+              (* TODO: Rule out *)
               admit.
-        ** admit. (* Cannot prove this, need to rule out ForcedChoice *)
-        ** rewrite runState_bind.
-           match goal with | [ |- context[Monad.unless ?P] ] => destruct P eqn:Hunless end.
-           ++ unfold Monad.unless.
-              rewrite monad_then.
-              rewrite monad_applicative_pure.
-              rewrite monad_left_id.
-              rewrite monad_left_id.
-              rewrite onReject_liftRM_bind.
-              rewrite runState_gets.
-              match goal with | [ |- context[when ?P] ] => destruct P eqn:Hwhen end.
-              -- unfold when.
-                 unfold reject.
-                 rewrite onReject_throwE.
-                 simpl. 
-                 destruct s0. simpl. assumption.
-              -- unfold when. rewrite pure_then_RM.
-                 rewrite onReject_liftRM_then.
-                 unfold createEmptyCanister.
-                 rewrite runState_then.
-                 unfold modify. rewrite runState_state.
-                 unfold snd.
-                 rewrite onReject_return, runState_return.
-                 unfold setReqStatus.
-                 unfold modify. rewrite runState_state.
-                 unfold Base.op_z2218U__ in *.
-                 destruct s0.
-                 simpl.
-                 (* now need theory about member and insert *)
-                 (* and that derivedId is not nil *)
-                 admit.
+           -- unfold Monad.unless. destruct_match.
+              ++ rewrite monad_then.
+                 rewrite monad_applicative_pure.
+                 rewrite monad_left_id.
+                 apply ESP_return.
+                 subst R'; unfold op_z2218U__; simpl.
+                 admit. (* derived id is not null *)
+              ++ unfold reject.
+                 rewrite monad_then.
+                 rewrite throwE_bind'.
+                 apply ESP_throwE.
+        ** intros.
+           apply ESP_bind with (R := fun _  => True).
+           -- apply ESP_liftRM.
+              apply SP_gets.
+              apply SP_get.
+              intros. trivial.
+           -- intros ex _.
+              apply ESP_then; [|apply ESP_then].
+              ++ unfold when.
+                 destruct_match.
+                 *** unfold reject. apply ESP_throwE.
+                 *** rewrite monad_applicative_pure. apply ESP_return. trivial.
+              ++ apply ESP_liftRM.
+                 admit. (* todo *)
+              ++ apply ESP_return; trivial.
+      - (* install request *)
+        admit.
+      - (* upgrade request *)
+        admit.
+      - (* update call request *) 
+        admit.
+    + (* pop message *)
+      admit.
 Admitted.
